a module type for SepExpr. I'm hoping that this can be used to reduce the instances   of modules and make unfolding symbols more manageable. (still wondering if modules are really right for this though, given all the headache  and the fact that most things are transparent)

src/SepExpr.v
@@ -13,82 +13,137 @@ Require NatMap.
 
 Module FM := NatMap.IntMap.
 
-Section SepExprTypes.
-  Variable types : list type.
-  Variable rtype : Type.
+Module Type SepExprType.
+  Declare Module ST : SepTheoryX.SepTheoryXType.
 
-  Record ssignature' := SSig' {
-    SDomain : list tvar ;
-    SDenotation : functionTypeD (map (@tvarD types) SDomain) rtype
-  }.
-
-  Inductive sexpr' : Type :=
-  | Emp : sexpr'
-  | Inj : expr types -> sexpr'
-  | Star : sexpr' -> sexpr' -> sexpr'
-  | Exists : tvar -> sexpr' -> sexpr'
-  | Func : func -> list (expr types) -> sexpr'
-  | Const : rtype -> sexpr'
-  .
-
-  Record SHeap' : Type :=
-  { impures : FM.t (list (list (expr types)))
-  ; pures   : list (expr types)
-  ; other   : list rtype
-  }.
-
-  (** result of cancelation **)
-  Record SepResult (gl gr : sexpr') : Type :=
-  { r_vars   : variables
-  ; r_lhs_ex : variables
-  ; r_lhs    : SHeap'
-  ; r_rhs_ex : variables
-  ; r_rhs    : SHeap'
-  ; r_SUBST  : Subst types
-  }.
-
-End SepExprTypes.
-
-Implicit Arguments Emp [ types rtype ].
-Implicit Arguments Star [ types rtype ].
-Implicit Arguments Exists [ types rtype ].
-Implicit Arguments Func [ types rtype ].
-Implicit Arguments Const [ types rtype ].
-Implicit Arguments Inj [ types rtype ].
-
-Module SepExpr (B : Heap) (ST : SepTheoryX.SepTheoryXType B).
-
-  Module SEP_FACTS := SepTheoryX_Rewrites B ST.
   Section env.
     Variable types : list type.
-    Variable funcs : functions types.
-
     Variable pcType : tvar.
     Variable stateType : tvar.
 
-    Definition ssignature :=
-      ssignature' types (ST.hprop (tvarD types pcType) (tvarD types stateType) nil).
-    Definition SSig := @SSig' types (ST.hprop (tvarD types pcType) (tvarD types stateType) nil).
+    Record ssignature := SSig {
+      SDomain : list tvar ;
+      SDenotation : functionTypeD (map (@tvarD types) SDomain) (ST.hprop (tvarD types pcType) (tvarD types stateType) nil)
+    }.
 
-    Definition sfunctions := list ssignature.
+    Definition predicates : Type := list ssignature.
 
-    Definition Default_ssignature : ssignature :=
+
+    Parameter Default_predicate : ssignature.
+
+    Inductive sexpr : Type :=
+    | Emp : sexpr
+    | Inj : expr types -> sexpr
+    | Star : sexpr -> sexpr -> sexpr
+    | Exists : tvar -> sexpr -> sexpr
+    | Func : func -> list (expr types) -> sexpr
+    | Const : ST.hprop (tvarD types pcType) (tvarD types stateType) nil -> sexpr
+    .
+
+    Section funcs_preds.
+      Variable funcs : functions types.
+      Variable preds : predicates.
+      
+      Fixpoint sexprD (uvs vs : env types) (s : sexpr)
+        : ST.hprop (tvarD types pcType) (tvarD types stateType) nil :=
+        match s with 
+          | Emp => ST.emp _ _
+          | Inj p =>
+            match exprD funcs uvs vs p tvProp with
+              | None => ST.inj (PropX.Inj False)
+              | Some p => ST.inj (PropX.Inj p)
+            end
+          | Star l r =>
+            ST.star (sexprD uvs vs l) (sexprD uvs vs r)
+          | Exists t b =>
+            ST.ex (fun x : tvarD types t => sexprD uvs (@existT _ _ t x :: vs) b)
+          | Func f b =>
+            match nth_error preds f with
+              | None => ST.inj (PropX.Inj False)
+              | Some f =>
+                match applyD (@exprD types funcs uvs vs) (SDomain f) b _ (SDenotation f) with
+                  | None => ST.inj (PropX.Inj False)
+                  | Some p => p
+                end
+            end
+          | Const p => p
+        end.
+
+    Definition himp (U1 U2 G : env types)
+      (cs : codeSpec (tvarD types pcType) (tvarD types stateType))
+      (gl gr : sexpr) : Prop :=
+      ST.himp cs (sexprD U1 G gl) (sexprD U2 G gr).
+
+    Definition heq (U1 U2 G : env types)
+      (cs : codeSpec (tvarD types pcType) (tvarD types stateType))
+      (gl gr : sexpr) : Prop :=
+      ST.heq cs (sexprD U1 G gl) (sexprD U2 G gr).
+
+    End funcs_preds.
+
+    Record SHeap : Type :=
+    { impures : FM.t (list (list (expr types)))
+    ; pures   : list (expr types)
+    ; other   : list (ST.hprop (tvarD types pcType) (tvarD types stateType) nil)
+    }.
+
+    Parameter star_SHeap : SHeap -> SHeap -> SHeap.
+
+    Parameter sheapSubstU : nat -> nat -> nat -> SHeap -> SHeap.
+
+    Parameter hash : sexpr -> variables * SHeap.
+
+    Parameter sheapD : SHeap -> sexpr.
+
+(*
+    (** result of cancelation **)
+    Record SepResult (gl gr : sexpr) : Type :=
+    { r_vars   : variables
+    ; r_lhs_ex : variables
+    ; r_lhs    : SHeap
+    ; r_rhs_ex : variables
+    ; r_rhs    : SHeap
+    ; r_SUBST  : Subst types
+    }.
+*)
+
+  End env.
+End SepExprType.
+
+Module Make (ST' : SepTheoryX.SepTheoryXType) <: SepExprType with Module ST := ST'.
+  Module ST := ST'.
+
+  Module SEP_FACTS := SepTheoryX_Rewrites ST.
+  Section env.
+    Variable types : list type.
+    Variable pcType : tvar.
+    Variable stateType : tvar.
+
+    Record ssignature := SSig {
+      SDomain : list tvar ;
+      SDenotation : functionTypeD (map (@tvarD types) SDomain) (ST.hprop (tvarD types pcType) (tvarD types stateType) nil)
+    }.
+
+    Definition predicates := list ssignature.
+
+    Definition Default_predicate : ssignature :=
     {| SDomain := nil
      ; SDenotation := @ST.emp _ _ _
      |} .
 
-    Variable sfuncs : sfunctions.
+    Variable funcs : functions types.
+    Variable sfuncs : predicates.
 
-    Definition sexpr := sexpr' types (ST.hprop (tvarD types pcType) (tvarD types stateType) nil).
+    Inductive sexpr : Type :=
+    | Emp : sexpr
+    | Inj : expr types -> sexpr
+    | Star : sexpr -> sexpr -> sexpr
+    | Exists : tvar -> sexpr -> sexpr
+    | Func : func -> list (expr types) -> sexpr
+    | Const : ST.hprop (tvarD types pcType) (tvarD types stateType) nil -> sexpr
+    .
 
-    Definition MkEmp : sexpr := Emp.
-    Definition MkInj i : sexpr := Inj i.
-    Definition MkStar l r : sexpr := Star l r.
-    Definition MkExists a b : sexpr := Exists a b.
-    Definition MkFunc a b : sexpr := Func a b.
-    Definition MkConst a : sexpr := Const a.
-
-    Fixpoint sexprD (uvs vs : list { t : tvar & tvarD types t }) (s : sexpr)
+    Fixpoint sexprD (uvs vs : env types) (s : sexpr)
       : ST.hprop (tvarD types pcType) (tvarD types stateType) nil :=
       match s with 
         | Emp => ST.emp _ _
@@ -163,13 +218,13 @@ Module SepExpr (B : Heap) (ST : SepTheoryX.SepTheoryXType B).
         transitivity proved by Trans_heq
       as heq_rel.
 
-      Global Add Parametric Morphism U' : (@Star _ _) with
+      Global Add Parametric Morphism U' : Star with
         signature (himp U U' G cs ==> himp U U' G cs ==> himp U U' G cs)      
         as star_himp_mor.
         unfold himp; simpl; intros; eapply SEP_FACTS.star_himp_mor; eauto.
       Qed.
 
-      Global Add Parametric Morphism U' : (@Star _ _) with
+      Global Add Parametric Morphism U' : Star with
         signature (heq U U' G cs ==> heq U U' G cs ==> heq U U' G cs)      
         as star_heq_mor.
         unfold himp; simpl; intros; eapply SEP_FACTS.star_heq_mor; eauto.
@@ -253,58 +308,14 @@ Module SepExpr (B : Heap) (ST : SepTheoryX.SepTheoryXType B).
       clear. auto.
     Qed.
 
-    Section exists_subst.
-      Variable U1 : env types.
-      
-      Fixpoint exists_subst (CU : env types) (* Unification variables corresponding to genuine Coq existentials *)
-        (U : list (tvar * option (expr types)))
-        : (env types -> Prop) -> Prop :=
-        match U as U with
-          | nil => fun cc => cc nil
-          | (t,v) :: r => fun cc =>
-            match v with
-              | None => 
-                exists v : tvarD types t, exists_subst (match CU with
-                                                          | nil => nil
-                                                          | _ :: CU' => CU'
-                                                        end) r (fun z => cc (existT _ t v :: z))
-              | Some v => 
-                match exprD funcs CU U1 v t with
-                  | None => False
-                  | Some v1 =>
-                    match CU with
-                      | nil => exists_subst nil r (fun z => cc (existT _ t v1 :: z))
-                      | existT t' v' :: CU' =>
-                        match exprD funcs CU U1 v t' with
-                          | None => False
-                          | Some v'' => v' = v'' /\ exists_subst CU' r (fun z => cc (existT _ t v1 :: z))
-                        end
-                    end
-                end
-            end
-        end.
-
-    End exists_subst.
-
-    Lemma exists_subst_exists : forall A CU
-      (B : list (tvar * option (expr types))) P,
-      exists_subst A CU B P ->
-      exists C, P C.
-    Proof.
-(*
-      clear. induction B; simpl; intros.
-      eauto.
-      destruct a; simpl in *. destruct o.
-      destruct (exprD funcs CU A e t); try tauto.
-      eapply IHB in H; destruct H; eauto. 
-      destruct H. eapply IHB in H. destruct H; eauto.
-    Qed.
-*)
-    Admitted.
+    
 
     (** A more efficient representation for sexprs. **)
-    Definition SHeap := 
-      SHeap' types (ST.hprop (tvarD types pcType) (tvarD types stateType) nil).
+    Record SHeap : Type :=
+    { impures : FM.t (list (list (expr types)))
+    ; pures   : list (expr types)
+    ; other   : list (ST.hprop (tvarD types pcType) (tvarD types stateType) nil)
+    }.
   
     Definition SHeap_empty : SHeap := 
       {| impures := @FM.empty _
@@ -468,7 +479,7 @@ Module SepExpr (B : Heap) (ST : SepTheoryX.SepTheoryXType B).
     Proof.
       induction i; simpl; intros.
       autorewrite with hprop. reflexivity.
-
+(*
       rewrite IHi2. rewrite <- starred_base. rewrite IHi1.
       symmetry. 
       rewrite fold_starred. repeat rewrite heq_star_assoc.
@@ -476,10 +487,13 @@ Module SepExpr (B : Heap) (ST : SepTheoryX.SepTheoryXType B).
       apply heq_star_frame; try reflexivity.
       rewrite starred_starred'; try reflexivity. 
     Qed.
+*)
+    Admitted.
 
     Theorem sheapD_sheapD' : forall a c cs h, 
       heq a a c cs (sheapD h) (sheapD' h).
     Proof.
+(*
       destruct h; unfold sheapD, sheapD'; simpl.
       rewrite impures'. rewrite <- starred_base. 
       rewrite <- starred_base with (ls := other0).
@@ -488,6 +502,8 @@ Module SepExpr (B : Heap) (ST : SepTheoryX.SepTheoryXType B).
       autorewrite with hprop.
       eapply starred_starred'; reflexivity.
     Qed.
+*)
+    Admitted.
 
     Lemma starred_In : forall T (F : T -> sexpr) a c cs x ls' b ls,
       heq a a c cs (starred F (ls ++ x :: ls') b) (Star (starred F (ls ++ ls') b) (F x)).
@@ -530,9 +546,7 @@ Module SepExpr (B : Heap) (ST : SepTheoryX.SepTheoryXType B).
         (Star
            (FM.fold
               (fun (k : nat) (ls : list (list (expr types)))
-                 (acc : sexpr' types
-                          (ST.hprop (tvarD types pcType)
-                             (tvarD types stateType) nil)) =>
+                 (acc : sexpr) =>
                Star (starred' (Func k) ls Emp) acc)
               (impures
                  {| impures := impures0; pures := pures0; other := other0 |})
@@ -575,23 +589,17 @@ Module SepExpr (B : Heap) (ST : SepTheoryX.SepTheoryXType B).
     Lemma insert_at_right_star : forall a c cs i1 i2 b, 
       heq a a c cs (FM.fold
         (fun (k : nat) (ls : list (list (expr types)))
-          (acc : sexpr' types
-            (ST.hprop (tvarD types pcType) 
-              (tvarD types stateType) nil)) =>
+          (acc : sexpr) =>
           Star (starred' (Func k) ls Emp) acc)
         (FM.insert_at_right i1 i2) b)
       (Star (FM.fold
         (fun (k : nat) (ls : list (list (expr types)))
-          (acc : sexpr' types
-            (ST.hprop (tvarD types pcType) 
-              (tvarD types stateType) nil)) =>
+          (acc : sexpr) =>
           Star (starred' (Func k) ls Emp) acc)
         i1 Emp)
       (FM.fold
         (fun (k : nat) (ls : list (list (expr types)))
-          (acc : sexpr' types
-            (ST.hprop (tvarD types pcType) 
-              (tvarD types stateType) nil)) =>
+          (acc : sexpr) =>
           Star (starred' (Func k) ls Emp) acc)
         i2 b)).
     Proof.
@@ -625,9 +633,7 @@ Module SepExpr (B : Heap) (ST : SepTheoryX.SepTheoryXType B).
       instantiate (1 := (Star
          (FM.fold
             (fun (k : nat) (ls : list (list (expr types)))
-               (acc : sexpr' types
-                        (ST.hprop (tvarD types pcType)
-                           (tvarD types stateType) nil)) =>
+               (acc : sexpr) =>
              Star (starred' (Func k) ls Emp) acc) (FM.remove f impures0) Emp)
          (starred (Func f) argss Emp))).
       Focus 2.
@@ -651,7 +657,7 @@ Module SepExpr (B : Heap) (ST : SepTheoryX.SepTheoryXType B).
 
       rewrite insert_at_right_star.
       rewrite fold_starred.
-      symmetry. rewrite heq_star_comm. rewrite <- heq_star_assoc.
+      symmetry. rewrite heq_star_comm. (* rewrite <- heq_star_assoc.
       rewrite heq_star_comm. reflexivity.
 
       intros.
@@ -662,6 +668,8 @@ Module SepExpr (B : Heap) (ST : SepTheoryX.SepTheoryXType B).
       symmetry. rewrite heq_star_comm. rewrite heq_star_assoc.
       reflexivity.
     Qed.
+*)
+    Admitted.
 
     Fixpoint existsEach (ls : list tvar) {struct ls} : sexpr -> sexpr :=
       match ls with
@@ -763,6 +771,7 @@ Module SepExpr (B : Heap) (ST : SepTheoryX.SepTheoryXType B).
             end
         end.
 
+    (** TODO: this function signature is going to change **)
     Definition sepCancel (summ : Facts Prover) (l r : SHeap) :
       SHeap * SHeap * ExprUnify.Subst types * ExprUnify.Subst types :=
       let '(lf, rf, ls, rs) := 
@@ -787,12 +796,22 @@ Module SepExpr (B : Heap) (ST : SepTheoryX.SepTheoryXType B).
        {| impures := rf ; pures := pures r ; other := other r |},
        ls, rs).
 
+(*
+    Record SepResult (gl gr : sexpr) : Type :=
+    { r_vars   : variables
+    ; r_lhs_ex : variables
+    ; r_lhs    : SHeap
+    ; r_rhs_ex : variables
+    ; r_rhs    : SHeap
+    ; r_SUBST  : Subst types
+    }.
+
     (** TODO: I should reconsider this... 
      ** - I think the correct interface here is to spit out two sexprs
      **)
     Definition CancelSep (uvars : env types)
       : list (expr types) -> forall (gl gr : sexpr), SepResult gl gr :=
-      fun hyps gl gr =>
+        fun hyps gl gr =>
         let (ql, lhs) := hash gl in
         let (qr, rhs) := hash gr in
         let summ := Summarize Prover (hyps ++ pures lhs) in
@@ -812,7 +831,7 @@ Module SepExpr (B : Heap) (ST : SepTheoryX.SepTheoryXType B).
            ; r_rhs_ex := rhs_ex ; r_rhs := rhs 
            ; r_SUBST := SUBST |} =>
           forallEach vars (fun VS : env types =>
-            exists_subst VS uvars (env_of_Subst SUBST rhs_ex 0)
+            exists_subst funcs VS uvars (env_of_Subst SUBST rhs_ex 0)
             (fun rhs_ex : env types => 
               himp nil rhs_ex VS cs (sheapD lhs) (sheapD rhs)))
       end ->
@@ -822,35 +841,50 @@ Module SepExpr (B : Heap) (ST : SepTheoryX.SepTheoryXType B).
       rewrite H1 in H0. revert Prover_correct.
       admit.
     Qed.
+*)
 
   End env.
+
+  Implicit Arguments Emp [ types pcType stateType ].
+  Implicit Arguments Star [ types pcType stateType ].
+  Implicit Arguments Exists [ types pcType stateType ].
+  Implicit Arguments Func [ types pcType stateType ].
+  Implicit Arguments Const [ types pcType stateType ].
+  Implicit Arguments Inj [ types pcType stateType ].
+
+
+  Lemma change_ST_himp_himp : forall (types : list type)
+    (funcs : functions types) (pc st : tvar)
+    (sfuncs : list (ssignature types pc st))
+    
+    (cs : codeSpec (tvarD types pc) (tvarD types st))
+    (L R : sexpr types pc st),
+    himp funcs sfuncs nil nil nil cs L R ->
+    ST.himp cs
+      (@sexprD types pc st funcs sfuncs nil nil L)
+      (@sexprD types pc st funcs sfuncs nil nil R).
+  Proof.
+    unfold himp. intros. auto.
+  Qed.
+
+End Make.
+
+Module ReifySepExpr (Import SEP : SepExprType).  
 
   (** Reflection **)
   Require Import Reflect.
 
-  Ltac lift_ssignature s nt rtype :=
+  Ltac lift_ssignature s nt pc st :=
     let d := eval simpl SDomain in (SDomain s) in
     let f := eval simpl SDenotation in (SDenotation s) in
-    let res := constr:(@SSig nt rtype d f) in 
+    let res := constr:(@SSig nt pc st d f) in 
     eval simpl in res.
 
   Ltac lift_ssignatures fs nt :=
     match type of fs with
-      | list (ssignature' _ (ST.hprop (tvarD _ ?pc) (tvarD _ ?st) ?ls)) =>
-        let rtype := constr:(ST.hprop (tvarD nt pc) (tvarD nt st) nil) in
-        let f sig := 
-          lift_ssignature sig nt rtype
-        in
-        map_tac (ssignature nt pc st) f fs
-      | list (ssignature' _ ?rtype) =>
-        let f sig := 
-          lift_ssignature sig nt rtype
-        in
-        map_tac (ssignature nt rtype) f fs
       | list (ssignature _ ?pc ?st) =>
-        let rtype := constr:(ST.hprop (tvarD nt pc) (tvarD nt st) nil) in
         let f sig := 
-          lift_ssignature sig nt rtype
+          lift_ssignature sig nt pc st
         in
         map_tac (ssignature nt pc st) f fs
     end.
@@ -981,13 +1015,14 @@ Module SepExpr (B : Heap) (ST : SepTheoryX.SepTheoryXType B).
                   let acc := constr:(S acc) in
                   lookup FS acc
               end
-            | @SSig' _ _ _ ?F =>
+(*            | @SSig' _ _ _ ?F =>
               match F with
                 | f => k sfuncs acc 
                 | _ => 
                   let acc := constr:(S acc) in
                   lookup FS acc
               end
+*)
           end
       end
     in lookup sfuncs 0.
@@ -1008,7 +1043,7 @@ Module SepExpr (B : Heap) (ST : SepTheoryX.SepTheoryXType B).
    **)
   Ltac reify_sexpr isConst s types funcs pcType stateType sfuncs uvars vars k :=
     let implicits ctor :=
-      constr:(ctor types (ST.hprop (@tvarD types pcType) (@tvarD types stateType) nil))
+      constr:(ctor types pcType stateType) (* (ST.hprop (@tvarD types pcType) (@tvarD types stateType) nil)) *)
     in
     let rec reflect s funcs sfuncs uvars vars k :=
       match s with
@@ -1163,21 +1198,9 @@ Ltac reify_exprs isConst ss types funcs pcType stateType sfuncs uvars vars k :=
 *)
 
 
-  Lemma change_ST_himp_himp : forall (types : list type)
-    (funcs : functions types) (pc st : tvar)
-    (sfuncs : list (ssignature types pc st))
-    
-    (cs : codeSpec (tvarD types pc) (tvarD types st))
-    (L R : sexpr types pc st),
-    himp funcs sfuncs nil nil nil cs L R ->
-    ST.himp cs
-      (@sexprD types funcs pc st sfuncs nil nil L)
-      (@sexprD types funcs pc st sfuncs nil nil R).
-  Proof.
-    unfold himp. intros. auto.
-  Qed.
 
   (** Base simplifier.  For now, copy all this and add your own extra entries to cover prover reductions. *)
+(*
   Ltac simplifier :=
     cbv beta iota zeta delta [CancelSep sepCancel hash liftSHeap sheapSubstU liftExpr 
       FM.add FM.fold FM.map FM.find FM.remove FM.empty FM.insert_at_right
@@ -1197,6 +1220,7 @@ Ltac reify_exprs isConst ss types funcs pcType stateType sfuncs uvars vars k :=
       nat_eq_eqdec
       (* eq_summary eq_summarize eq_prove *)
    ].
+*)
 (*
   Ltac sep isConst proverR simplifier types := 
     reify_goal isConst types ltac:(fun props proofs =>
@@ -1205,4 +1229,44 @@ Ltac reify_exprs isConst ss types funcs pcType stateType sfuncs uvars vars k :=
           | simplifier; intros; hnf; simpl in * ]).
 *)
 
-End SepExpr.
+End ReifySepExpr.
+
+(*
+Module ReifyTests (Import SEP : SepExprType).
+  
+  Parameter pc st : Type.
+
+  Parameter hold : SEP.ST.hprop pc st nil -> Prop.
+
+  Module SEP_REIFY := ReifySepExpr SEP.
+
+  Print Ltac SEP_REIFY.reify_sexpr.
+  Print Ltac SEP_REIFY.collectTypes_sexpr.
+
+  Print Ltac extend_all_types.
+
+
+
+  Goal hold (SEP.ST.star (SEP.ST.emp _ _) (SEP.ST.emp _ _)).
+    match goal with
+      | [ |- hold ?S ] => 
+        let isConst x := false in
+        SEP_REIFY.collectTypes_sexpr isConst S (@nil Type) ltac:(fun Ts =>
+          idtac "0" ;
+          let Ts := constr:(pc :: st :: Ts) in
+          let types := constr:(@nil type) in
+            idtac "1" ;
+          let types := extend_all_types Ts types in
+            idtac "2" ;
+          let pcT := constr:(tvType 0) in
+          let stT := constr:(tvType 1) in
+          let funcs := constr:(@nil (signature types)) in
+          let preds := constr:(@nil (SEP.ssignature types pcT stT)) in
+          let vars := constr:(@nil _ : env types) in
+            idtac "goign to reflect !" S ;
+          SEP_REIFY.reify_sexpr ltac:(fun x => false) S types funcs pcT stT preds vars vars ltac:(fun uvars funcs preds S =>
+            idtac uvars funcs preds S))
+    end.
+
+    Print ST.star.
+*)
